specs/lib/fst/Spec.Lib.IntBuf.fst
@@ -55,6 +55,38 @@ let salloc #h0 #a #b #len clen init read writes spec impl =
   pop_frame();
   r
 
+let salloc11 #h0 #a #b #c #len #wlen clen init read write spec impl =
+  push_frame();
+  let buf = create clen init in
+  let r = impl buf in
+  let inv (h1:mem) (j:nat) = True in
+  let f' (j:size_t{0 <= v j /\ v j <= len}) : Stack unit
+      (requires (fun h -> inv h (v j)))
+      (ensures (fun h1 _ h2 -> inv h2 (v j + 1))) =
+      upd #a #len buf j init in
+  Spec.Lib.Loops.for (size 0) clen inv f';
+  pop_frame();
+  r
+
+let salloc21 #h0 #a0 #a1 #b #w #len0 #len1 #wlen clen0 clen1 init0 init1 reads write spec impl =
+  push_frame();
+  let buf0 = create clen0 init0 in
+  let buf1 = create clen1 init1 in
+  let r = impl buf0 buf1 in
+  let inv (h1:mem) (j:nat) = True in
+  let f'0 (j:size_t{0 <= v j /\ v j <= len0}) : Stack unit
+      (requires (fun h -> inv h (v j)))
+      (ensures (fun h1 _ h2 -> inv h2 (v j + 1))) =
+      upd #a0 #len0 buf0 j init0 in
+  let f'1 (j:size_t{0 <= v j /\ v j <= len1}) : Stack unit
+      (requires (fun h -> inv h (v j)))
+      (ensures (fun h1 _ h2 -> inv h2 (v j + 1))) =
+      upd #a1 #len1 buf1 j init1 in
+  Spec.Lib.Loops.for (size 0) clen0 inv f'0;
+  Spec.Lib.Loops.for (size 0) clen1 inv f'1;
+  pop_frame();
+  r
+
 let map #a #len clen f b =
   let h0 = ST.get() in
   let inv (h1:mem) (j:nat) = True in
